\documentclass[11pt]{article}
\usepackage[utf8]{inputenc}
\usepackage[T1]{fontenc}     % Fix weird character
\usepackage{geometry}
\usepackage{amsmath}
\usepackage{amssymb}
\usepackage{gensymb}
\usepackage{spalign}
\usepackage{xfrac}
\usepackage{parskip}
\usepackage{float}  % figure[H]
\usepackage[style=ieee,backend=biber]{biblatex}
\usepackage[breaklinks=true,bookmarks=true,hidelinks]{hyperref}
\usepackage{tikz}
\usepackage{enumitem}

\geometry{
    a4paper,
    hmargin=2.54cm,
    tmargin=1.27cm,
    bmargin=1.27cm,
    includeheadfoot
}
\setcounter{secnumdepth}{0}  % Disable section numbering

\begin{document}
Lös ekvationen $x \cdot y' = (y - 1)^{3/2}$ för begynnelsevärdenna

\begin{enumerate}[label=\roman*.]
    \item $y(1) = 2$
    \item $y(1) = 1$
\end{enumerate}

\noindent\rule{\textwidth}{0.5pt}

Lösning:

\begin{equation}
    x \cdot y' = (y - 1)^{3/2} = \frac{dy}{dx}x = (y - 1)^{\frac{3}{2}}
\end{equation}

\begin{align}
    \frac{dy}{dx}x = (y - 1)^{\frac{3}{2}} &\Leftrightarrow xdy = (y - 1)^{\frac{3}{2}}dx \\
    &\Leftrightarrow (y - 1)^{-\frac{3}{2}}dy = x^{-1}dx
\end{align}

\begin{align}
    \int (y - 1)^{-\frac{3}{2}}dy &= \int x^{-1}dx \\
    -2\frac{1}{(y - 1)^{\frac{1}{2}}} &= \ln x + C \\
    -2\frac{1}{\ln x + C} &= (y - 1)^{\frac{1}{2}} \\
    (y - 1)^{\frac{1}{2}} &= -2\frac{1}{\ln x + C}\\
    y - 1 &= \left(-\frac{2}{\ln x + C}\right)^2\\
    y &= \left(-\frac{2}{\ln x + C}\right)^2 + 1\\
\end{align}

För $y(1) = 2$

\begin{align}
    2 &= \left(-\frac{2}{\ln 1 + C}\right)^2 + 1\\
    2 &= \frac{4}{C^2} + 1\\
    1 &= \frac{4}{C^2} \\
    C^2 &= 4 \\
    C &= \sqrt{4} = 2 \\
\end{align}

För $y(1) = 1$

\begin{align}
    1 &= \left(-\frac{2}{\ln 1 + C}\right)^2 + 1\\
    1 &= \frac{4}{C^2} + 1\\
    0 &= \frac{4}{C^2} \\
\end{align}

\end{document}

